chore: make formula.lean use predicates on assns

Lean/Geo/SAT/Formula.lean
@@ -4,7 +4,7 @@ import Mathlib.Data.Fintype.Prod
 /-! The CNF that we produce, as a `PropFun`. -/
 
 namespace Geo
-open LeanSAT Model
+open LeanSAT Model PropFun
 
 inductive Var (n : Nat)
   | sigma  (a b c : Fin n)
@@ -12,7 +12,7 @@ inductive Var (n : Nat)
   | hole   (a b c : Fin n)
   deriving DecidableEq
 
-def signotopeAxiom (a b c d : Fin n) : PropFun (Var n) :=
+def orientationConstraint (a b c d : Fin n) : PropFun (Var n) :=
   let sabc := Var.sigma a b c
   let sacd := Var.sigma a c d
   let sabd := Var.sigma a b d
@@ -24,122 +24,50 @@ def signotopeAxiom (a b c d : Fin n) : PropFun (Var n) :=
     (¬{sabc} ∧ ¬{sbcd} → ¬{sacd})
   ]
 
-/-- Asserts that orientation constraints are satisfied.
+def orientationConstraints (n : Nat) : PropAssignment (Var n) → Prop :=
+  fun τ => ∀ a b c d, a < b → b < c → c < d →
+    τ ⊨ orientationConstraint a b c d
 
-  ∀ 1 ≤ a < b < c ≤ n:
-    ∀ {d}, c < d:
-      !s{a, b, c} ∨ !s{a, c, d} ∨  s{a, b, d} ≃ (s{a, b, c} ∧ s{a, c, d}) → s{a, b, d}
-      !s{a, b, c} ∨ !s{b, c d}  ∨  s{a, c, d} ≃ (s{a, b, c} ∧ s{b, c, d}) → s{a, c, d}
-
-      (We take the top grouping and do them again, except negating the actual variables)
-
-       s{a, b, c} ∨  s{a, c, d} ∨ !s{a, b, d} ≃ (!s{a, b, c} ∧ !s{a, c, d}) → !s{a, b, d}
-       s{a, b, c} ∨  s{b, c, d} ∨ !s{a, c, d} ≃ (!s{a, b, c} ∧ !s{b, c, d}) → !s{a, c, d} -/
-def signotopeAxioms (n : Nat) : PropFun (Var n) :=
-  let U : Multiset (Fin n) := Finset.univ.val
-  PropFun.all (U.map (fun a =>
-    PropFun.all (U.map fun b =>
-      PropFun.all (U.map fun c =>
-        PropFun.all (U.map fun d =>
-          if a < b ∧ b < c ∧ c < d then signotopeAxiom a b c d else ⊤)))))
-
-def xIsInsideDef (a b c x : Fin n) : PropFun (Var n) :=
+def xIsInsideDef (a b c x : Fin n) : PropAssignment (Var n) → Prop := fun τ =>
   let sabc := Var.sigma a b c
   let saxc := Var.sigma a x c
   let saxb := Var.sigma a x b
   let sbxc := Var.sigma b x c
   let I := Var.inside x a b c
-  if a < x ∧ x < b then
-    [propfun| {I} ↔ (({sabc} ↔ {saxc}) ∧ (¬{saxb} ↔ {sabc})) ]
-  else if b < x ∧ x < c then
-    [propfun| {I} ↔ (({sabc} ↔ {saxc}) ∧ (¬{sbxc} ↔ {sabc})) ]
-  else
-    ⊤
+  ( a < x → x < b →
+    τ ⊨ [propfun| {I} ↔ (({sabc} ↔ {saxc}) ∧ (¬{saxb} ↔ {sabc})) ]
+  ) ∧ (
+    b < x → x < c →
+    τ ⊨ [propfun| {I} ↔ (({sabc} ↔ {saxc}) ∧ (¬{sbxc} ↔ {sabc})) ]
+  )
 
-/-- Defines "is inside triangle" variables.
-
-  (We split on whether the candidate point "x" to be inside is before or after "b")
-
-  ∀ {x}, a < x < b:
-    I{x, a, b, c} ↔ ((s{a, b, c} ↔ s{a, x, c}) ∧ (!s{a, x, b} ↔ s{a, b, c}))
-
-  ∀ {x}, b < x < c:
-    I{x, a, b, c} ↔ ((s{a, b, c} ↔ s{a, x, c}) ∧ (!s{b, x, c} ↔ s{a, b, c})) -/
-def insideDefs (n : Nat) : PropFun (Var n) :=
-  let U : Multiset (Fin n) := Finset.univ.val
-  PropFun.all (U.map (fun a =>
-    PropFun.all (U.map fun b =>
-      PropFun.all (U.map fun c =>
-        PropFun.all (U.map fun x =>
-          if a < b ∧ b < c then
-            xIsInsideDef a b c x
-          else
-            ⊤)))))
-
-def notHoleOfPointInside (a b c : Fin n) : PropFun (Var n) :=
-  let U : Multiset (Fin n) := Finset.univ.val
-  PropFun.all (U.map (fun x =>
-    if a < x ∧ x < c ∧ x ≠ b then
-      [propfun| {Var.inside x a b c} → ¬{Var.hole a b c} ]
-    else
-      ⊤))
-
-def hasPointInside (a b c : Fin n) : PropFun (Var n) :=
-  let U : Multiset (Fin n) := Finset.univ.val
-  PropFun.any (U.map (fun x =>
-    if a < x ∧ x < c ∧ x ≠ b then
-      Var.inside x a b c
-    else
-      ⊥))
-
-/-- Defines "is hole" variables.
-
-    ∀ {a b c x}, a < x < c, with x ≠ b:
-      I{x, a, b, c} → !H{a, b, c}
-
-    !H{a, b, c} → ⋁_{a < x < c, x ≠ b} I{x, a, b, c}
-
-  (Triangle abc is not a hole iff some x is inside triangle abc.) -/
-def holeDefs (n : Nat) : PropFun (Var n) :=
-  let U : Multiset (Fin n) := Finset.univ.val
-  PropFun.all (U.map (fun a =>
-    PropFun.all (U.map fun b =>
-      PropFun.all (U.map fun c =>
-        if a < b ∧ b < c then
-          [propfun|
-            {notHoleOfPointInside a b c} ∧
-            (¬{Var.hole a b c} → {hasPointInside a b c})
-          ]
-        else
-          ⊤))))
+/-- Defines "is inside triangle" variables. -/
+def insideDefs (n : Nat) : PropAssignment (Var n) → Prop := fun τ =>
+  ∀ a b c, a < b → b < c →
+    ∀ x, (τ |> xIsInsideDef a b c x)
 
 /-- Defines "is hole" variables.
 
   Triangle abc is a hole iff all x are not inside triangle abc. -/
-def holeDefs' (n : Nat) : PropAssignment (Var n) → Prop := fun τ =>
-  ∀ {a b c}, τ (Var.hole a b c) ↔
-    (∀ x, a < x → x < c → x ≠ b →
-      !τ (Var.inside x a b c))
+def holeDefs (n : Nat) : PropAssignment (Var n) → Prop := fun τ =>
+  ∀ {a b c}, a < b → b < c →
+    (τ (Var.hole a b c) ↔
+      (∀ x, a < x → x < c → x ≠ b → !τ (Var.inside x a b c)))
 
 /-- Asserts that no holes exist. -/
-def noHoles (n : Nat) : PropFun (Var n) :=
-  let U : Multiset (Fin n) := Finset.univ.val
-  PropFun.all (U.map (fun a =>
-    PropFun.all (U.map fun b =>
-      PropFun.all (U.map fun c =>
-        if a < b ∧ b < c then
-          (Var.hole a b c)ᶜ
-        else ⊤))))
+def noHoles (n : Nat) : PropAssignment (Var n) → Prop := fun τ =>
+  ∀ a b c, a < b → b < c → !τ (Var.hole a b c)
 
--- Symmetry breaking that the leftmost point is CCW with respect to any two other sorted points
-def pointsCCW (n : Nat) : PropFun (Var n) :=
-  let U : Multiset (Fin n) := Finset.univ.val
-  PropFun.all (U.map (fun a =>
-    PropFun.all (U.map fun b =>
-      if ⟨0, Fin.size_positive a⟩ < a ∧ a < b then
-        Var.sigma ⟨0, Fin.size_positive a⟩ a b
-      else
-        ⊤)))
+/-- Symmetry breaking that the leftmost point is CCW with respect to any two other sorted points -/
+def pointsCCW (n : Nat) : PropAssignment (Var n) → Prop := fun τ =>
+  ∀ a b,
+    have : NeZero n := ⟨by have := Fin.size_positive a; aesop⟩
+    0 < a → a < b → τ (Var.sigma 0 a b)
 
-def theFormula (n : Nat) : PropFun (Var n) :=
-  signotopeAxioms n ⊓ insideDefs n ⊓ holeDefs n ⊓ noHoles n ⊓ pointsCCW n
+/-- The abstract formula encoding empty triangle on `n` points. -/
+def theFormula (n : Nat) : PropAssignment (Var n) → Prop := fun τ =>
+  (τ |> orientationConstraints n) ∧
+  (τ |> insideDefs n) ∧
+  (τ |> holeDefs n) ∧
+  (τ |> noHoles n) ∧
+  (τ |> pointsCCW n)
