Lean/Geo/SAT/WBAssn.lean
@@ -18,8 +18,8 @@ noncomputable def toPropAssn (w : WBPoints) : PropAssignment (Var w.length)
   | .inside x a b c .. => decide $ σPtInTriangle w[x] w[a] w[b] w[c]
   | .hole a b c ..     => decide $ σIsEmptyTriangleFor w[a] w[b] w[c] w.toFinset
 
-theorem satisfies_signotopeAxiom (w : WBPoints) (i j k l : Fin w.length) :
-    i < j → j < k → k < l → w.toPropAssn ⊨ signotopeAxiom i j k l := by
+theorem satisfies_orientationConstraint (w : WBPoints) (i j k l : Fin w.length) :
+    i < j → j < k → k < l → w.toPropAssn ⊨ orientationConstraint i j k l := by
   intro hij hjk hkl
   have : [w[i], w[j], w[k], w[l]] <+ w.points := by
     have : [w[i], w[j], w[k], w[l]] = [i,j,k,l].map w.points.get := by
@@ -31,7 +31,7 @@ theorem satisfies_signotopeAxiom (w : WBPoints) (i j k l : Fin w.length) :
   have s : Sorted₄ w[i] w[j] w[k] w[l] := w.sorted.to₄ this
   have gp : InGeneralPosition₄ w[i] w[j] w[k] w[l] :=
     PointListInGeneralPosition.to₄ w.gp this
-  simp only [signotopeAxiom, satisfies_conj, satisfies_impl, satisfies_var,
+  simp only [orientationConstraint, satisfies_conj, satisfies_impl, satisfies_var,
     toPropAssn, decide_eq_true_eq, and_imp, satisfies_neg]
   constructor
   . exact σ_prop₂ s gp
@@ -43,14 +43,12 @@ theorem satisfies_signotopeAxiom (w : WBPoints) (i j k l : Fin w.length) :
   . simp_rw [gp.gp₁.σ_iff, gp.gp₄.σ_iff, gp.gp₃.σ_iff]
     exact σ_prop₃ s gp
 
-theorem satisfies_signotopeAxioms (w : WBPoints) : w.toPropAssn ⊨ signotopeAxioms w.length := by
-  unfold signotopeAxioms
-  simp only [signotopeAxioms, satisfies_all, Multiset.mem_map, Finset.mem_val, Finset.mem_univ, true_and,
+theorem satisfies_orientationConstraints (w : WBPoints) : w.toPropAssn |> orientationConstraints w.length := by
+  unfold toPropAssn
+  simp only [orientationConstraints, satisfies_all, Multiset.mem_map, Finset.mem_val, Finset.mem_univ, true_and,
     forall_exists_index, forall_apply_eq_imp_iff]
-  intro i j k l
-  split
-  . apply satisfies_signotopeAxiom <;> tauto
-  exact satisfies_tr
+  intros
+  apply satisfies_orientationConstraint <;> assumption
 
 theorem insideDefs_aux₁ {a x b c : Point} : Sorted₄ a x b c → InGeneralPosition₄ a x b c →
     (σPtInTriangle x a b c ↔
@@ -89,138 +87,146 @@ theorem insideDefs_aux₂ {a b x c : Point} : Sorted₄ a b x c → InGeneralPos
     rw [σ_prop₃ sorted gp h₁ h₄] at h₃
     contradiction
 
-theorem satisfies_insideDefs (w : WBPoints) : w.toPropAssn ⊨ insideDefs w.length := by
+theorem satisfies_insideDefs (w : WBPoints) : w.toPropAssn |> insideDefs w.length := by
   unfold insideDefs xIsInsideDef
   simp only [satisfies_all, Multiset.mem_map, forall_exists_index, forall_apply_eq_imp_iff, Finset.mem_val,
     Finset.mem_univ, true_and]
-  intro a b c x
-  split_ifs <;> first | exact satisfies_tr | unfold toPropAssn
-  next abc axb =>
+  intro a b c hab hbc x
+  constructor
+  · intro hax hxb
     have : [w[a], w[x], w[b], w[c]] <+ w.points := by
       have : [w[a], w[x], w[b], w[c]] = [a,x,b,c].map w.points.get := by
         simp [GetElem.getElem, List.getElem_eq_get]
       rw [this]
       apply map_get_sublist
-      simp [abc.left, axb.left, abc.left.trans abc.right, axb.right, axb.right.trans abc.right, abc.right]
-    simp [-getElem_fin, insideDefs_aux₁ (w.sorted.to₄ this) (PointListInGeneralPosition.to₄ w.gp this) ]
-  next abc _ bxc =>
+      have : a < c := hab.trans hbc
+      have : x < c := hxb.trans hbc
+      simp [*]
+    simp [toPropAssn, -getElem_fin]
+    exact insideDefs_aux₁ (w.sorted.to₄ this) (PointListInGeneralPosition.to₄ w.gp this)
+  · intro hbx hxc
     have : [w[a], w[b], w[x], w[c]] <+ w.points := by
       have : [w[a], w[b], w[x], w[c]] = [a,b,x,c].map w.points.get := by
         simp [GetElem.getElem, List.getElem_eq_get]
       rw [this]
       apply map_get_sublist
-      simp [abc.left, abc.left.trans bxc.left, abc.left.trans abc.right, bxc.left, abc.right, bxc.right]
-    simp [-getElem_fin, insideDefs_aux₂ (w.sorted.to₄ this) (PointListInGeneralPosition.to₄ w.gp this)]
+      have : a < x := hab.trans hbx
+      have : a < c := hab.trans hbc
+      simp [*]
+    simp [toPropAssn, -getElem_fin]
+    exact insideDefs_aux₂ (w.sorted.to₄ this) (PointListInGeneralPosition.to₄ w.gp this)
 
+/-- There used to be a declaration in `Formula.lean` called
+`notHoleOfPointInside`; it is just one direction of `holeDefs` -/
 theorem satisfies_notHoleOfPointInside (w : WBPoints) (a b c : Fin w.length) :
-    w.toPropAssn ⊨ notHoleOfPointInside a b c := by
-  unfold notHoleOfPointInside
+    (∃ x, w.toPropAssn (Var.inside x a b c)) → ¬ w.toPropAssn (Var.hole a b c) := by
   simp only [satisfies_all, Multiset.mem_map, forall_exists_index, forall_apply_eq_imp_iff, Finset.mem_val, Finset.mem_univ, true_and]
   intro x
-  split_ifs <;> try exact satisfies_tr
-  simp only [satisfies_impl, satisfies_var, satisfies_neg, decide_eq_true_eq, toPropAssn, σIsEmptyTriangleFor,
-    not_forall, not_not, exists_prop, toFinset, List.mem_toFinset, coe_toFinset, Set.mem_setOf_eq]
+  simp only [toPropAssn, decide_eq_true_eq, σIsEmptyTriangleFor, toFinset, coe_toFinset,
+    Set.mem_setOf_eq, not_forall, not_not, exists_prop]
   intro h
   exact ⟨w[x], List.get_mem _ x _, h⟩
 
 theorem satisfies_hasPointInside (w : WBPoints) (a b c : Fin w.length) :
     a < b → b < c →
-    w.toPropAssn ⊨ [propfun| (¬{Var.hole a b c} → {hasPointInside a b c}) ] := by
+    ¬ w.toPropAssn (Var.hole a b c) → ∃ x, a < x ∧ x < c ∧ x ≠ b ∧ w.toPropAssn (Var.inside x a b c) := by
   intro ab bc
-  unfold toPropAssn hasPointInside σIsEmptyTriangleFor
-  simp only [ne_eq, satisfies_impl, satisfies_neg, satisfies_var, decide_eq_true_eq,
-    not_forall, not_not, exists_prop, satisfies_any, Multiset.mem_map, Finset.mem_val,
-    Finset.mem_univ, true_and, exists_exists_eq_and, forall_exists_index, and_imp]
+  unfold toPropAssn σIsEmptyTriangleFor
+  simp only [Finset.mem_coe, getElem_fin, decide_eq_true_eq, not_forall, not_not, exists_prop,
+    forall_exists_index, and_imp]
   intro x hx tri
   rcases List.get_of_mem <| List.mem_toFinset.mp hx with ⟨i, rfl⟩
   have : List.get w.points i = w[i] := rfl
   rw [this] at tri hx
   clear this
   use i
-  split_ifs
-  . simp only [satisfies_var, decide_eq_true_eq, tri]
-  next h =>
-    exfalso
-    simp only [not_and, not_not] at h
-    have sub : [w[a],w[b],w[c]] <+ w.points := by
-      have : [w[a],w[b],w[c]] = [a,b,c].map w.points.get := by
-        simp [GetElem.getElem, List.getElem_eq_get]
-      rw [this]
-      apply map_get_sublist
-      aesop (add unsafe lt_trans)
-    have ia : i ≠ a := fun h => by
-      rw [h] at tri
-      have := not_mem_σPtInTriangle (w.gp sub).perm₁
-      have := tri.perm₁
-      contradiction
-    have ic : i ≠ c := fun h => by
-      rw [h] at tri
-      have := not_mem_σPtInTriangle (w.gp sub).perm₂
-      have := tri.perm₂
-      contradiction
-    have : InGeneralPosition₄ w[i] w[a] w[b] w[c] := tri.gp₄_of_gp₃ (w.gp sub)
-    have ⟨wawi, wiwc⟩ := xBounded_of_PtInTriangle (w.sorted.to₃ sub) ((σPtInTriangle_iff this).mp tri)
-    have : w[a].x < w[i].x := by
-      apply lt_of_le_of_ne wawi
-      intro h
-      exact ia <| w.of_eqx h.symm
-    have ai : a < i := w.of_sorted_get this
-    have : w[i].x < w[c].x := by
-      apply lt_of_le_of_ne wiwc
-      intro h
-      exact ic <| w.of_eqx h
-    have ic : i < c := w.of_sorted_get this
-    rw [h ai ic] at tri
-    apply not_mem_σPtInTriangle (w.gp sub) tri
+  have sub : [w[a],w[b],w[c]] <+ w.points := by
+    have : [w[a],w[b],w[c]] = [a,b,c].map w.points.get := by
+      simp [GetElem.getElem, List.getElem_eq_get]
+    rw [this]
+    apply map_get_sublist
+    aesop (add unsafe lt_trans)
+  have ia : i ≠ a := fun h => by
+    rw [h] at tri
+    have := not_mem_σPtInTriangle (w.gp sub).perm₁
+    have := tri.perm₁
+    contradiction
+  have ib : i ≠ b := fun h => by
+    rw [h] at tri
+    have := not_mem_σPtInTriangle (w.gp sub).perm₁.perm₁
+    contradiction
+  have ic : i ≠ c := fun h => by
+    rw [h] at tri
+    have := not_mem_σPtInTriangle (w.gp sub).perm₂
+    have := tri.perm₂
+    contradiction
+  have : InGeneralPosition₄ w[i] w[a] w[b] w[c] := tri.gp₄_of_gp₃ (w.gp sub)
+  have ⟨wawi, wiwc⟩ := xBounded_of_PtInTriangle (w.sorted.to₃ sub) ((σPtInTriangle_iff this).mp tri)
+  have : w[a].x < w[i].x := by
+    apply lt_of_le_of_ne wawi
+    intro h
+    exact ia <| w.of_eqx h.symm
+  have ai : a < i := w.of_sorted_get this
+  have : w[i].x < w[c].x := by
+    apply lt_of_le_of_ne wiwc
+    intro h
+    exact ic <| w.of_eqx h
+  have ic : i < c := w.of_sorted_get this
+  simp_all
 
-theorem satisfies_holeDefs (w : WBPoints) : w.toPropAssn ⊨ holeDefs w.length := by
+theorem satisfies_holeDefs (w : WBPoints) : w.toPropAssn |> holeDefs w.length := by
   simp [holeDefs]
-  intro a b c
-  split_ifs <;> try exact satisfies_tr
-  next h =>
-    simp only [satisfies_conj, satisfies_notHoleOfPointInside, satisfies_hasPointInside _ _ _ _ h.left h.right, true_and]
+  intro a b c hab hbc
+  constructor
+  · intro h x _ _ _
+    have := satisfies_notHoleOfPointInside w a b c
+    rw [imp_not_comm] at this
+    specialize this h
+    simp at this
+    apply this
+  · intro h
+    by_contra contra
+    have ⟨x,hax,hxc,hxb,hinside⟩ := satisfies_hasPointInside w a b c hab hbc contra
+    specialize h x hax hxc hxb
+    rw [h] at hinside
+    contradiction
 
-theorem satisfies_leftmostCCWDefs (w : WBPoints) : w.toPropAssn ⊨ pointsCCW w.length := by
+theorem satisfies_leftmostCCWDefs (w : WBPoints) : w.toPropAssn |> pointsCCW w.length := by
   unfold pointsCCW
   simp
-  intro i j
-  split <;> try exact satisfies_tr
-  next h =>
-    have ⟨k, hk⟩ : ∃ k, i.1 = k + 1 := by
-      apply Nat.exists_eq_succ_of_ne_zero
-      have : 0 < i.1 := h.left
-      linarith
-    have ⟨l, hl⟩ : ∃ l, j.1 = l + 1 := by
-      apply Nat.exists_eq_succ_of_ne_zero
-      have : 0 < j.1 := h.left.trans h.right
-      linarith
-    unfold toPropAssn
-    cases i
-    cases j
-    simp at hk hl
-    simp [GetElem.getElem, points, hk, hl]
-    apply List.pairwise_iff_get.mp w.oriented
-    simp at h ⊢
+  intro i j h0i hij
+  have ⟨k, hk⟩ : ∃ k, i.1 = k + 1 := by
+    apply Nat.exists_eq_succ_of_ne_zero
+    have : 0 < i.1 := h0i
     linarith
+  have ⟨l, hl⟩ : ∃ l, j.1 = l + 1 := by
+    apply Nat.exists_eq_succ_of_ne_zero
+    have : 0 < j.1 := h0i.trans hij
+    linarith
+  unfold toPropAssn
+  cases i
+  cases j
+  simp at hk hl
+  simp [GetElem.getElem, points, hk, hl]
+  apply List.pairwise_iff_get.mp w.oriented
+  simp at *
+  linarith
 
 theorem satisfies_noHoles (w : WBPoints) :
     ¬σHasEmptyTriangle w.toFinset →
-    w.toPropAssn ⊨ theFormula w.length := by
+    (w.toPropAssn |> theFormula w.length) := by
   unfold theFormula
   intro noholes
-  simp only [noHoles, satisfies_conj, satisfies_signotopeAxioms, satisfies_insideDefs, and_self,
+  simp only [noHoles, satisfies_conj, satisfies_orientationConstraints, satisfies_insideDefs, and_self,
     satisfies_holeDefs, satisfies_all, Multiset.mem_map, Finset.mem_val, Finset.mem_univ, true_and,
     forall_exists_index, forall_apply_eq_imp_iff, satisfies_leftmostCCWDefs, and_true]
-  intro a b c
-  split_ifs
-  next h =>
-    unfold toPropAssn
-    simp only [satisfies_neg, satisfies_var, decide_eq_true_eq]
-    simp only [σHasEmptyTriangle, not_exists, not_and] at noholes
-    apply noholes _ (w.get_mem_toFinset a) _ (w.get_mem_toFinset b) _ (w.get_mem_toFinset c)
-      (fun h' => ne_of_lt h.left <| (w.of_eqx <| congrArg (·.x) h'))
-      (fun h' => ne_of_lt (h.left.trans h.right) <| (w.of_eqx <| congrArg (·.x) h'))
-      (fun h' => ne_of_lt h.right <| (w.of_eqx <| congrArg (·.x) h'))
-  . exact satisfies_tr
+  intro a b c hab hbc
+  unfold toPropAssn
+  simp only [getElem_fin, Bool.not_eq_true', decide_eq_false_iff_not]
+  simp only [σHasEmptyTriangle, not_exists, not_and] at noholes
+  apply noholes _ (w.get_mem_toFinset a) _ (w.get_mem_toFinset b) _ (w.get_mem_toFinset c)
+    (fun h' => ne_of_lt hab <| (w.of_eqx <| congrArg (·.x) h'))
+    (fun h' => ne_of_lt (hab.trans hbc) <| (w.of_eqx <| congrArg (·.x) h'))
+    (fun h' => ne_of_lt hbc <| (w.of_eqx <| congrArg (·.x) h'))
 
 end WBPoints
